WIP

src/localdrfra/RARace.v
@@ -45,6 +45,12 @@ Module ReleaseWrites.
         Memory.get loc to lc.(Local.promises) = None /\
         exists from val released,
           Memory.get loc to mem = Some (from, Message.concrete val released).
+
+    Lemma append_app e rels1 rels2:
+      append e rels1 ++ rels2 = append e (rels1 ++ rels2).
+    Proof.
+      unfold append. des_ifs.
+    Qed.
   End ReleaseWrites.
 End ReleaseWrites.
 
@@ -60,22 +66,36 @@ Module RATrace.
     | thread_steps_step
         rels pf e e1 e2 e3
         (STEPS: @thread_steps lang rels e1 e2)
-        (STEP: @OrdThread.step lang L Ordering.acqrel pf e e2 e3)
-        (SILENT: ThreadEvent.get_machine_event e = MachineEvent.silent):
+        (STEP: @OrdThread.step lang L Ordering.acqrel pf e e2 e3):
         thread_steps lang (ReleaseWrites.append L e rels) e1 e3
     .
+    Hint Constructors thread_steps.
+
+    Inductive thread_tau_steps lang: forall (rels: ReleaseWrites.t) (e1 e2: Thread.t lang), Prop :=
+    | thread_tau_steps_refl
+        e:
+        thread_tau_steps lang [] e e
+    | thread_tau_steps_step
+        rels pf e e1 e2 e3
+        (STEPS: @thread_tau_steps lang rels e1 e2)
+        (STEP: @OrdThread.step lang L Ordering.acqrel pf e e2 e3)
+        (SILENT: ThreadEvent.get_machine_event e = MachineEvent.silent):
+        thread_tau_steps lang (ReleaseWrites.append L e rels) e1 e3
+    .
+    Hint Constructors thread_steps.
 
     Inductive configuration_step: forall (e: MachineEvent.t) (tid: Ident.t) (rels: ReleaseWrites.t) (c1 c2: Configuration.t), Prop :=
     | configuration_step_intro
         rels
         pf e tid c1 lang st1 lc1 e2 st3 lc3 sc3 memory3
         (TID: IdentMap.find tid c1.(Configuration.threads) = Some (existT _ lang st1, lc1))
-        (STEPS: thread_steps lang rels (Thread.mk _ st1 lc1 c1.(Configuration.sc) c1.(Configuration.memory)) e2)
+        (STEPS: thread_tau_steps lang rels (Thread.mk _ st1 lc1 c1.(Configuration.sc) c1.(Configuration.memory)) e2)
         (STEP: OrdThread.step L Ordering.acqrel pf e e2 (Thread.mk _ st3 lc3 sc3 memory3))
         (CONSISTENT: OrdThread.consistent L Ordering.acqrel (Thread.mk _ st3 lc3 sc3 memory3)):
         configuration_step (ThreadEvent.get_machine_event e) tid (ReleaseWrites.append L e rels)
                            c1 (Configuration.mk (IdentMap.add tid (existT _ _ st3, lc3) c1.(Configuration.threads)) sc3 memory3)
     .
+    Hint Constructors configuration_step.
 
     Inductive configuration_steps: forall (rels: ReleaseWrites.t) (c1 c2: Configuration.t), Prop :=
     | configuration_steps_refl
@@ -87,10 +107,41 @@ Module RATrace.
         (STEP: configuration_step e tid rels' c2 c3):
         configuration_steps (rels' ++ rels) c1 c3
     .
+    Hint Constructors configuration_steps.
 
-    Lemma thread_steps_rtc_tau_step
+    Lemma thread_tau_steps_steps
           lang rels e1 e2
-          (STEPS: thread_steps lang rels e1 e2):
+          (STEPS: thread_tau_steps lang rels e1 e2):
+      thread_steps lang rels e1 e2.
+    Proof.
+      induction STEPS; eauto.
+    Qed.
+
+    Lemma thread_steps_app
+          lang rels1 rels2 e1 e2 e3
+          (STEPS1: thread_steps lang rels1 e1 e2)
+          (STEPS2: thread_steps lang rels2 e2 e3):
+      thread_steps lang (rels2 ++ rels1) e1 e3.
+    Proof.
+      revert rels1 e1 STEPS1. induction STEPS2; i; eauto.
+      exploit IHSTEPS2; eauto. i.
+      rewrite ReleaseWrites.append_app. econs 2; eauto.
+    Qed.
+
+    Lemma thread_tau_steps_app
+          lang rels1 rels2 e1 e2 e3
+          (STEPS1: thread_tau_steps lang rels1 e1 e2)
+          (STEPS2: thread_tau_steps lang rels2 e2 e3):
+      thread_tau_steps lang (rels2 ++ rels1) e1 e3.
+    Proof.
+      revert rels1 e1 STEPS1. induction STEPS2; i; eauto.
+      exploit IHSTEPS2; eauto. i.
+      rewrite ReleaseWrites.append_app. econs 2; eauto.
+    Qed.
+
+    Lemma thread_tau_steps_rtc_tau_step
+          lang rels e1 e2
+          (STEPS: thread_tau_steps lang rels e1 e2):
       rtc (@OrdThread.tau_step lang L Ordering.acqrel) e1 e2.
     Proof.
       induction STEPS; eauto.
@@ -103,7 +154,7 @@ Module RATrace.
           (STEP: configuration_step e tid rels c1 c2):
       OrdConfiguration.step L Ordering.acqrel e tid c1 c2.
     Proof.
-      inv STEP. exploit thread_steps_rtc_tau_step; eauto. i.
+      inv STEP. exploit thread_tau_steps_rtc_tau_step; eauto. i.
       destruct (ThreadEvent.get_machine_event e0) eqn:EVENT.
       - rewrite <- EVENT. econs 2; eauto. destruct e0; ss.
       - rewrite <- EVENT. econs 2; eauto. destruct e0; ss.
@@ -124,16 +175,17 @@ Module RARace.
        <<ORDR: Ordering.le ordr Ordering.strong_relaxed>>).
 
     Definition racefree (s: Threads.syntax): Prop :=
-      forall rels c
+      forall rels1 c
         tid lang st1 lc1
-        pf loc to val released ord e2 e3
-        (CSTEPS: RATrace.configuration_steps L rels (Configuration.init s) c)
+        rels2 pf loc to val released ord e2 e3
+        (CSTEPS: RATrace.configuration_steps L rels1 (Configuration.init s) c)
         (TID: IdentMap.find tid c.(Configuration.threads) = Some (existT _ lang st1, lc1))
-        (STEPS: rtc (@OrdThread.tau_step lang L Ordering.acqrel)
-                    (Thread.mk _ st1 lc1 c.(Configuration.sc) c.(Configuration.memory)) e2)
+        (STEPS: RATrace.thread_steps L lang rels2
+                                     (Thread.mk _ st1 lc1 c.(Configuration.sc) c.(Configuration.memory))
+                                     e2)
         (CONS: Local.promise_consistent e2.(Thread.local))
         (STEP: OrdThread.step L Ordering.acqrel pf (ThreadEvent.read loc to val released ord) e2 e3)
-        (RACE: ra_race rels e2.(Thread.local).(Local.tview) loc to ord),
+        (RACE: ra_race (rels2 ++ rels1) e2.(Thread.local).(Local.tview) loc to ord),
         False.
   End RARace.
 End RARace.
